src/l0/L0.X509.AliasKeyTBS.Extensions.fst
@@ -196,8 +196,8 @@ let lemma_serialize_aliasKeyTBS_extensions_payload_size x
                                               x.aliasKeyTBS_extensions_basicConstraints;
     lemma_serialize_aliasKeyTBS_extensions_authKeyID_size_exact
                                               x.aliasKeyTBS_extensions_authKeyID;
-    lemma_serialize_l0_extension_size_exact x.aliasKeyTBS_extensions_riot;
-  lemma_length_of_aliasKeyTBS_extensions_payload_size_max x.aliasKeyTBS_extensions_l0.x509_extValue_riot.riot_version
+    lemma_serialize_l0_extension_size_exact x.aliasKeyTBS_extensions_l0;
+  lemma_length_of_aliasKeyTBS_extensions_payload_size_max x.aliasKeyTBS_extensions_l0.x509_extValue_l0.riot_version
 
 
 (*
